formal-proofs/theories/lib/concurrent_linked_list/list_spec.v
@@ -1,0 +1,78 @@
+From SegmentQueue.lib.concurrent_linked_list Require Export segment_spec.
+From iris.program_logic Require Import atomic.
+From iris.heap_lang Require Export proofmode notation lang.
+Open Scope nat.
+
+Record listSpec Σ `{!heapG Σ} {impl: segmentInterface}
+       (segment_spec: segmentSpec Σ impl) :=
+  ListSpec {
+      list_name: Type;
+      is_concurrentLinkedList: namespace -> list_name -> iProp Σ;
+      is_concurrentLinkedList_persistent N γ:
+        Persistent (is_concurrentLinkedList N γ);
+      segment_in_list
+        (γ: list_name)
+        (γs: linkedListNode_name _ _ (linkedListNode_base _ _ segment_spec))
+        (id: nat)
+        (v: val): iProp Σ;
+      segment_in_list_persistent γ γs id v:
+        Persistent (segment_in_list γ γs id v);
+      segment_is_cancelled: list_name -> nat -> iProp Σ;
+      segment_is_cancelled_persistent γ id:
+        Persistent (segment_is_cancelled γ id);
+      pointer_location: list_name -> loc -> nat -> iProp Σ;
+      newList: val;
+      cleanPrev: val;
+      findSegment: val;
+      moveForward: val;
+      onSlotCleaned: val;
+      newList_spec N (k: nat):
+        {{{ ⌜k > 0⌝ }}}
+          newList #k
+        {{{ γ ℓ, RET #ℓ; is_concurrentLinkedList N γ ∗
+                        [∗ list] i ∈ seq 0 k,
+                            pointer_location γ (ℓ +ₗ (i: nat)) 0
+        }}};
+      findSegment_spec N γ γs' (start_id id: nat) v:
+        {{{ is_concurrentLinkedList N γ ∗ segment_in_list γ γs' start_id v }}}
+          findSegment v #id
+        {{{ (v': val) (id': nat), RET (SOMEV v');
+          (∃ γs, segment_in_list γ γs id' v')
+          ∗ ⌜(start_id ≤ id' ∧ id ≤ id')%nat⌝
+          ∗ ∀ i, (⌜max start_id id ≤ i < id'⌝)%nat -∗ segment_is_cancelled γ i
+        }}};
+      moveForward_spec N γ γs (ℓ: loc) id v:
+        is_concurrentLinkedList N γ -∗
+        segment_in_list γ γs id v -∗
+        <<< ∀ id', ▷ pointer_location γ ℓ id' >>>
+          moveForward #ℓ v @ ⊤ ∖ ↑N
+        <<< ∃ (r: bool), if r then pointer_location γ ℓ (max id id')
+                              else ▷ pointer_location γ ℓ id'
+                                   ∗ segment_is_cancelled γ id,
+            RET #r >>>;
+      cleanPrev_spec N γ γs id ptr:
+        {{{ is_concurrentLinkedList N γ ∗ segment_in_list γ γs id ptr }}}
+          cleanPrev ptr
+        {{{ RET #(); True }}};
+      onSlotCleaned_spec N Ψ γ γs id p:
+        is_concurrentLinkedList N γ -∗
+        segment_in_list γ γs id p -∗
+        <<< (∀ n, segment_content _ _ segment_spec γs id n ==∗
+            Ψ ∗ ∃ n', ⌜(n = S n')%nat⌝ ∧
+                      segment_content _ _ segment_spec γs id n') >>>
+          onSlotCleaned p @ ⊤ ∖ ↑N
+        <<< Ψ, RET #() >>>;
+      pointer_location_load γ (ℓ: loc):
+        ⊢ <<< ∀ id, ▷ pointer_location γ ℓ id >>>
+          ! #ℓ @ ⊤
+        <<< ∃ γs p, pointer_location γ ℓ id ∗ segment_in_list γ γs id p,
+            RET p >>>;
+      access_segment N (known_is_removed: bool) E γ γs id ptr:
+        ↑N ⊆ E ->
+        is_concurrentLinkedList N γ -∗
+        segment_in_list γ γs id ptr -∗
+        (if known_is_removed then segment_is_cancelled γ id else True) -∗
+        |={E, E ∖ ↑N}=> ∃ n, ⌜known_is_removed = false ∨ n = 0⌝ ∧
+                            ▷ segment_content _ _ _ γs id n ∗
+                            (▷ segment_content _ _ _ γs id n ={E ∖ ↑N, E}=∗ emp);
+    }.
